commutativity2.thy
@@ -39,10 +39,10 @@ lemma sessionsInTransactionEmpty:
 lemma sessionsInTransactionEmptySnoc:
   "sessionsInTransaction (tr@[a]) i = (
 if i=length tr then
-  if \<exists>t ts. snd a = ABeginAtomic t ts then
-       sessionsInTransaction tr (length tr - 1) \<union> {fst a}
-  else if snd a = AEndAtomic then
-       sessionsInTransaction tr (length tr - 1) - {fst a}
+  if \<exists>t ts. get_action a = ABeginAtomic t ts then
+       sessionsInTransaction tr (length tr - 1) \<union> {get_invoc a}
+  else if get_action a = AEndAtomic then
+       sessionsInTransaction tr (length tr - 1) - {get_invoc a}
   else 
        sessionsInTransaction tr (length tr - 1)
 else if i > length tr then
@@ -52,9 +52,9 @@ else
 proof (intro if_cases2; clarsimp?)
   fix t ts
   assume a0: "i = length tr"
-    and a1: "snd a = ABeginAtomic t ts"
+    and a1: "get_action a = ABeginAtomic t ts"
 
-  then show "sessionsInTransaction (tr @ [a]) (length tr) = insert (fst a) (sessionsInTransaction tr (length tr - Suc 0))"
+  then show "sessionsInTransaction (tr @ [a]) (length tr) = insert (get_invoc a) (sessionsInTransaction tr (length tr - Suc 0))"
   proof (cases a, auto)
     show "\<And>aa x. \<lbrakk>a = (aa, ABeginAtomic t ts); i = length tr; x \<in> sessionsInTransaction (tr @ [(aa, ABeginAtomic t ts)]) (length tr); x \<notin> sessionsInTransaction tr (length tr - Suc 0)\<rbrakk> \<Longrightarrow> x = aa"
       apply (auto simp add: nth_append sessionsInTransaction_def inTransaction_def split: if_splits)[1]
@@ -67,9 +67,9 @@ proof (intro if_cases2; clarsimp?)
   qed
 next
   assume a0: "i = length tr"
-    and a1: "snd a = AEndAtomic"
+    and a1: "get_action a = AEndAtomic"
 
-  then show "sessionsInTransaction (tr @ [a]) (length tr) = sessionsInTransaction tr (length tr - Suc 0) - {fst a}"
+  then show "sessionsInTransaction (tr @ [a]) (length tr) = sessionsInTransaction tr (length tr - Suc 0) - {get_invoc a}"
     apply (cases a, auto)
       apply (auto simp add: nth_append sessionsInTransaction_def inTransaction_def split: if_splits)[1]
       apply (smt Suc_pred inc_induct less_Suc_eq less_imp_le_nat linorder_neqE_nat not_less_zero)
@@ -78,8 +78,8 @@ next
     by (metis Suc_pred leD le_SucI length_greater_0_conv less_Suc_eq_le list.size(3) not_less_zero)
 next
   assume a0: "i = length tr"
-    and a1: "\<forall>t ts. snd a \<noteq> ABeginAtomic t ts"
-    and a2: "snd a \<noteq> AEndAtomic"
+    and a1: "\<forall>t ts. get_action a \<noteq> ABeginAtomic t ts"
+    and a2: "get_action a \<noteq> AEndAtomic"
 
   then show "sessionsInTransaction (tr @ [a]) (length tr) = sessionsInTransaction tr (length tr - Suc 0)"
     apply (cases a, auto)
@@ -160,12 +160,12 @@ lemma packedTraces_stay_in_transaction:
   assumes steps: "S ~~ tr \<leadsto>* S'"
     and "packed_trace tr"
     and "currentTransaction S invoc \<triangleq> tx"
-    and "tr \<noteq> [] \<Longrightarrow> fst (hd tr) = invoc"
+    and "tr \<noteq> [] \<Longrightarrow> get_invoc (hd tr) = invoc"
     and "(invoc, AEndAtomic) \<notin> set tr"
     and "\<And>i. (i, AFail) \<notin> set tr"
-    and "\<And>a. a\<in>set tr \<Longrightarrow> \<not>allowed_context_switch (snd a)"
+    and "\<And>a. a\<in>set tr \<Longrightarrow> \<not>allowed_context_switch (get_action a)"
     and "j < length tr"
-  shows "currentTransaction S' invoc \<triangleq> tx \<and> fst (tr ! j) = invoc"
+  shows "currentTransaction S' invoc \<triangleq> tx \<and> get_invoc (tr ! j) = invoc"
   using assms proof (induct arbitrary: j rule: steps_induct)
   case initial
   then show ?case by auto
@@ -186,10 +186,10 @@ next
     then have [simp]: "packed_trace (x#xs)"
       by (simp add: local.Cons)
 
-    have [simp]: "currentTransaction S' (fst x) = Some tx"
+    have [simp]: "currentTransaction S' (get_invoc x) = Some tx"
       using local.Cons step.IH step.prems by force
 
-    have "fst (last tr) = invoc"
+    have "get_invoc (last tr) = invoc"
       using last_conv_nth local.Cons step.IH step.prems by fastforce
 
     from Cons step
@@ -200,8 +200,8 @@ next
       assume j_def[simp]: "j = length (x # xs)"
 
       from use_packed_trace[OF \<open>packed_trace (tr @ [a])\<close>, where i="length tr"]
-      have a_allowed_ctxt_switch: "fst a = invoc"
-        by (metis \<open>fst (last tr) = invoc\<close> diff_less j_def last_conv_nth length_greater_0_conv less_numeral_extra(1) list.simps(3) local.Cons nth_append_first nth_append_length nth_mem step.prems(6) step.prems(7)) 
+      have a_allowed_ctxt_switch: "get_invoc a = invoc"
+        by (metis \<open>get_invoc (last tr) = invoc\<close> diff_less j_def last_conv_nth length_greater_0_conv less_numeral_extra(1) list.simps(3) local.Cons nth_append_first nth_append_length nth_mem step.prems(6) step.prems(7)) 
 
       have ?thesis
         by (simp add: \<open>currentTransaction S'' invoc \<triangleq> tx\<close> a_allowed_ctxt_switch local.Cons) 
@@ -226,11 +226,11 @@ lemma packedTraces_transactions_same_invocation:
     and noFail: "\<And>i. (i, AFail) \<notin> set tr"
     and beginTx: "tr ! i = (invoc, ABeginAtomic tx txns)"
     and noEndTx: "\<forall>j. i < j \<and> j < k \<longrightarrow> tr ! j \<noteq> (invoc, AEndAtomic)"
-    and noContextSwitch: "\<forall>j. i < j \<and> j < k \<longrightarrow> \<not>allowed_context_switch (snd (tr!j))"
+    and noContextSwitch: "\<forall>j. i < j \<and> j < k \<longrightarrow> \<not>allowed_context_switch (get_action (tr!j))"
     and [simp]: "i < j" 
     and [simp]: "j < k"
     and [simp]: "k \<le> length tr"
-  shows "fst (tr ! j) = invoc"
+  shows "get_invoc (tr ! j) = invoc"
 proof -
   have "take (Suc i) tr @ drop (Suc i) (take k tr) @ drop k tr = tr"
     apply (auto simp add: drop_take append_eq_conv_conj min_def)
@@ -246,7 +246,7 @@ proof -
 
 
   from \<open>S1 ~~ drop (Suc i) (take k tr) \<leadsto>* S2\<close>
-  have "fst ( drop (Suc i) (take k tr) ! (j - Suc i)) = invoc"
+  have "get_invoc ( drop (Suc i) (take k tr) ! (j - Suc i)) = invoc"
   proof (rule packedTraces_stay_in_transaction2)
     show "packed_trace (drop (Suc i) (take k tr))"
       using \<open>packed_trace tr\<close> packed_trace_drop packed_trace_take by blast 
@@ -260,7 +260,7 @@ proof -
     then show  "currentTransaction S1 invoc \<triangleq> tx"
       using beginTx by (auto simp add: step_simps)
       
-    show  "drop (Suc i) (take k tr) \<noteq> [] \<Longrightarrow> fst (hd (drop (Suc i) (take k tr))) = invoc"
+    show  "drop (Suc i) (take k tr) \<noteq> [] \<Longrightarrow> get_invoc (hd (drop (Suc i) (take k tr))) = invoc"
       using \<open>packed_trace tr\<close> by (smt One_nat_def \<open>take (Suc i) tr @ drop (Suc i) (take k tr) @ drop k tr = tr\<close> append_Cons append_eq_append_conv append_is_Nil_conv append_self_conv append_take_drop_id \<open>i < j\<close> \<open>j < k\<close> \<open>k \<le> length tr\<close> beginTx diff_Suc_Suc diff_zero fst_conv hd_Cons_tl lessI less_trans_Suc noContextSwitch not_le_imp_less nth_via_drop packed_trace_def take_all zero_less_Suc)
       
     show  "(invoc, AEndAtomic) \<notin> set (drop (Suc i) (take k tr))"
@@ -269,7 +269,7 @@ proof -
     show  "\<And>ia. (ia, AFail) \<notin> set (drop (Suc i) (take k tr))"
       using noFail by (meson in_set_dropD in_set_takeD )
 
-    show  "\<And>a. a \<in> set (drop (Suc i) (take k tr)) \<Longrightarrow> \<not> allowed_context_switch (snd a)"
+    show  "\<And>a. a \<in> set (drop (Suc i) (take k tr)) \<Longrightarrow> \<not> allowed_context_switch (get_action a)"
       using noContextSwitch  apply (auto simp add: in_set_conv_nth take_nth drop_nth min_def  split: if_splits)
          apply (metis less_add_Suc1 snd_conv)
       apply (metis add.commute add_Suc assms(9) le_antisym less_add_Suc1 less_diff_conv snd_conv)
@@ -280,7 +280,7 @@ proof -
       by (simp add: Suc_leI diff_less_mono min.absorb2)
       
   qed
-  then show "fst (tr ! j) = invoc "
+  then show "get_invoc (tr ! j) = invoc "
     using assms(7) assms(8) assms(9) by auto
 qed
 
