examples.thy
@@ -9,7 +9,7 @@ text "Various examples to illustrate definitions."
 \<comment> \<open>counts how many concurrent transactions are active\<close>
 definition transactionsArePackedMeasure :: "('proc, 'operation, 'any) trace \<Rightarrow> nat" where
   "transactionsArePackedMeasure tr \<equiv>
-\<Sum>i\<in>{..<length tr}. card (sessionsInTransaction tr i - {fst (tr!i)})  "
+\<Sum>i\<in>{..<length tr}. card (sessionsInTransaction tr i - {get_invoc (tr!i)})  "
 
 
 theorem not_packed_example2:
@@ -20,16 +20,16 @@ theorem not_packed_example2:
   \<and> sessionsInTransaction tr i - {s} \<noteq> {}" (is ?goal)
 proof -
   from notPacked
-  have "0 < (\<Sum>i<length tr. card (sessionsInTransaction tr i - {fst (tr ! i)}))"
+  have "0 < (\<Sum>i<length tr. card (sessionsInTransaction tr i - {get_invoc (tr ! i)}))"
     by (auto simp add: transactionsArePackedMeasure_def)
   from this 
   obtain i 
     where a: "i < length tr" 
-      and b: "card (sessionsInTransaction tr i - {fst (tr ! i)}) > 0"
+      and b: "card (sessionsInTransaction tr i - {get_invoc (tr ! i)}) > 0"
     by (meson lessThan_iff not_less sum_nonpos)
 
   from b 
-  have "sessionsInTransaction tr i - {fst (tr!i)} \<noteq> {}"
+  have "sessionsInTransaction tr i - {get_invoc (tr!i)} \<noteq> {}"
     by fastforce
 
   then show ?thesis
